Restructure to remove ctxs from induction & various improvements

WIP/CutElim2.v
@@ -12,6 +12,25 @@ Module Notations.
 End Notations.
 Import Notations.
 
+
+(*TODO: move to Utils*)
+Lemma fresh_with_names_from [V' A B] v (c' : @NamedList.named_list V' A) (s : list B)
+  : Datatypes.length c' = Datatypes.length s -> fresh v (with_names_from c' s) = fresh v c'.
+Proof.
+  intros.
+  unfold fresh.
+  basic_utils_crush.
+Qed.
+Hint Rewrite fresh_with_names_from : utils.
+
+
+(*TODO: move to Rule.v*)
+Local Ltac use_rule_in_ws :=
+  match goal with
+  | H:ws_lang ?l, Hin:In (_, _) ?l |- _ => pose proof (rule_in_ws _ _ H Hin)
+  end.
+
+
 Section WithVar.
   Context (V : Type)
     {V_Eqb : Eqb V}
@@ -28,6 +47,59 @@ Section WithVar.
   Notation subst := (@subst V).
   Notation rule := (@rule V).
   Notation lang := (@lang V).
+
+
+(*TODO: move to term*)
+Lemma ws_subst_from_ws_args args (c' : ctx) (s : list term)
+  : length c' = length s ->
+    all_fresh c' ->
+    well_scoped args s ->
+    well_scoped args (with_names_from c' s).
+Proof.
+  revert c'; induction s;
+    destruct c';
+    basic_goal_prep;
+    basic_term_crush.
+  eapply IHs; eauto.
+Qed.
+Hint Resolve ws_subst_from_ws_args : lang_core.
+
+
+  (*TODO: move to Term *)
+  Lemma term_ws_incl (t:term) args args'
+    : well_scoped args t ->incl args args' -> well_scoped args' t.
+  Proof.
+    induction t;
+      basic_goal_prep;
+      basic_term_crush.
+    revert dependent l;
+      induction l;
+      basic_goal_prep;
+      basic_term_crush.
+  Qed.
+  
+  Lemma sort_ws_incl (t:sort) args args'
+    : well_scoped args t ->incl args args' -> well_scoped args' t.
+  Proof.
+    destruct t.
+    revert dependent l;
+      induction l;
+      basic_goal_prep;
+      basic_term_crush.
+    eapply term_ws_incl; eauto.
+  Qed.
+
+  
+  Lemma ws_ctx_in c n t
+    : ws_ctx c -> In (n,t) c -> well_scoped (map fst c) t.
+  Proof.
+    induction c;
+      basic_goal_prep;
+      basic_term_crush.
+    all:eapply sort_ws_incl; eauto.
+    all: basic_utils_crush.
+  Qed.
+  Hint Resolve ws_ctx_in : lang_core.
 
 
   Notation PreModel := (@PreModel V term sort).
@@ -54,6 +126,9 @@ Local Notation mut_mod eq_sort eq_term wf_sort wf_term :=
 Section Terms.
   Context (l : lang).
 
+  Section WithCtx.
+  Context (c : ctx).
+
   (*All assume wf_lang.
     All ctxs (other than in wf_ctx) are assumed to satisfy wf_ctx.
     Judgments whose assumptions take ctxs must ensure they are wf.
@@ -66,64 +141,65 @@ Section Terms.
      Currently have them duplicated, but ideally the ones in Model.v
      could be generalized to be usable here.
    *)
-  Inductive eq_sort : ctx -> sort -> sort -> Prop :=
-  | eq_sort_by : forall c name c' t1 t2 s1 s2,
+  Inductive eq_sort : sort -> sort -> Prop :=
+  | eq_sort_by : forall name c' t1 t2 s1 s2,
       In (name, sort_eq_rule c' t1 t2) l ->
-      eq_subst c c' s1 s2 ->
-      eq_sort c t1[/s1/] t2[/s2/]
-  | eq_sort_cong : forall c name c' args s1 s2,
+      eq_subst c' s1 s2 ->
+      eq_sort t1[/s1/] t2[/s2/]
+  | eq_sort_cong : forall name c' args s1 s2,
       In (name,sort_rule c' args) l ->
-      eq_args c c' s1 s2 ->
-      eq_sort c (scon name s1) (scon name s2)
-  | eq_sort_trans : forall c t1 t12 t2,
-      eq_sort c t1 t12 ->
-      eq_sort c t12 t2 ->
-      eq_sort c t1 t2
-  | eq_sort_sym : forall c t1 t2, eq_sort c t1 t2 -> eq_sort c t2 t1
-  with eq_term : ctx -> sort -> term -> term -> Prop :=
-  | eq_term_by : forall c name c' t e1 e2 s1 s2,
+      eq_args c' s1 s2 ->
+      eq_sort (scon name s1) (scon name s2)
+  | eq_sort_trans : forall t1 t12 t2,
+      eq_sort t1 t12 ->
+      eq_sort t12 t2 ->
+      eq_sort t1 t2
+  | eq_sort_sym : forall t1 t2, eq_sort t1 t2 -> eq_sort t2 t1
+  with eq_term : sort -> term -> term -> Prop :=
+  | eq_term_by : forall name c' t e1 e2 s1 s2,
       In (name,term_eq_rule c' e1 e2 t) l ->
-      eq_subst c c' s1 s2 ->
-      eq_term c t[/s2/] e1[/s1/] e2[/s2/]
-  | eq_term_cong : forall c name c' args t s1 s2,
+      eq_subst c' s1 s2 ->
+      eq_term t[/s2/] e1[/s1/] e2[/s2/]
+  | eq_term_cong : forall name c' args t s1 s2,
       In (name,term_rule c' args t) l ->
-      eq_args c c' s1 s2 ->
-      eq_term c t[/(with_names_from c' s2)/] (con name s1) (con name s2)
-  | eq_term_var : forall c n t,
+      eq_args c' s1 s2 ->
+      eq_term t[/(with_names_from c' s2)/] (con name s1) (con name s2)
+  | eq_term_var : forall n t,
       In (n, t) c ->
-      eq_term c t (var n) (var n)
-  | eq_term_trans : forall c t e1 e12 e2,
-      eq_term c t e1 e12 ->
-      eq_term c t e12 e2 ->
-      eq_term c t e1 e2
-  | eq_term_sym : forall c t e1 e2, eq_term c t e1 e2 -> eq_term c t e2 e1
+      eq_term t (var n) (var n)
+  | eq_term_trans : forall t e1 e12 e2,
+      eq_term t e1 e12 ->
+      eq_term t e12 e2 ->
+      eq_term t e1 e2
+  | eq_term_sym : forall t e1 e2, eq_term t e1 e2 -> eq_term t e2 e1
   (* Conversion:
 
 c |- e1 = e2 : t 
                ||
 c |- e1 = e2 : t'
    *)
-  | eq_term_conv : forall c e1 e2 t t',
-      eq_term c t e1 e2 ->
-      eq_sort c t t' ->
-      eq_term c t' e1 e2
-  with eq_subst : ctx -> ctx -> subst -> subst -> Prop :=
-  | eq_subst_nil : forall c : ctx, eq_subst c [] [] []
-  | eq_subst_cons : forall (c c' : ctx) (s1 s2 : subst),
-                    eq_subst c c' s1 s2 ->
+  | eq_term_conv : forall e1 e2 t t',
+      eq_term t e1 e2 ->
+      eq_sort t t' ->
+      eq_term t' e1 e2
+  with eq_subst : ctx -> subst -> subst -> Prop :=
+  | eq_subst_nil : eq_subst [] [] []
+  | eq_subst_cons : forall (c' : ctx) (s1 s2 : subst),
+                    eq_subst c' s1 s2 ->
                     forall (name : V) (t : sort) (e1 e2 : term),
-                    eq_term c t [/s2 /] e1 e2 ->
-                    eq_subst c ((name, t) :: c') ((name, e1) :: s1)
+                    eq_term t [/s2 /] e1 e2 ->
+                    eq_subst ((name, t) :: c') ((name, e1) :: s1)
                       ((name, e2) :: s2)
-  with eq_args : ctx -> ctx -> list term -> list term -> Prop :=
-  | eq_args_nil : forall c : ctx, eq_args c [] [] []
-  | eq_args_cons : forall (c c' : ctx) (es1 es2 : list term),
-      eq_args c c' es1 es2 ->
+  with eq_args : ctx -> list term -> list term -> Prop :=
+  | eq_args_nil : eq_args [] [] []
+  | eq_args_cons : forall (c' : ctx) (es1 es2 : list term),
+      eq_args c' es1 es2 ->
       forall (name : V) (t : sort) (e1 e2 : term),
-        eq_term c t [/with_names_from c' es2 /] e1 e2 ->
-        eq_args c ((name, t) :: c') (e1 :: es1) (e2 :: es2).                
+        eq_term t [/with_names_from c' es2 /] e1 e2 ->
+        eq_args ((name, t) :: c') (e1 :: es1) (e2 :: es2).                
 
-  (* TODO: do I need these?
+  
+  (* TODO: do I need these? make notations for reflexivity
   Inductive wf_term : ctx -> term -> sort -> Prop :=
   | wf_term_by : forall c n s args c' t,
       In (n, term_rule c' args t) l ->
@@ -156,7 +232,7 @@ c |- e1 = e2 : t'
   Notation wf_args := (wf_args (Model:= cut_model)).
   Notation wf_ctx := (wf_ctx (Model:= cut_model)).
    *)
-  
+
   
   (* TODO: bug? This doesn't work even w/ eq_subst and eq_args defined mutually.
   Combined Scheme eq_ind
@@ -164,135 +240,135 @@ c |- e1 = e2 : t'
    *)    
   
   Section EqInd.
-    Context (P_sort : ctx -> sort -> sort -> Prop)
-      (P_term : ctx -> sort -> term -> term -> Prop)
-      (P_subst : ctx -> ctx -> subst -> subst -> Prop)
-      (P_args : ctx -> ctx -> list term -> list term -> Prop).
+    Context (P_sort : sort -> sort -> Prop)
+      (P_term : sort -> term -> term -> Prop)
+      (P_subst : ctx -> subst -> subst -> Prop)
+      (P_args : ctx -> list term -> list term -> Prop).
 
     (* sort hypotheses *)
-    Context (Hsort0 : forall (c c' : ctx) (name : V) t1 t2 s1 s2,
+    Context (Hsort0 : forall (c' : ctx) (name : V) t1 t2 s1 s2,
           In (name, sort_eq_rule c' t1 t2) l ->
-          eq_subst c c' s1 s2 ->
-          P_subst c c' s1 s2 ->
-          P_sort c t1[/s1/] t2[/s2/])
-      (Hsort1 : forall (c c' : ctx) (name : V) args s1 s2,
+          eq_subst c' s1 s2 ->
+          P_subst c' s1 s2 ->
+          P_sort t1[/s1/] t2[/s2/])
+      (Hsort1 : forall (c' : ctx) (name : V) args s1 s2,
           In (name, sort_rule c' args) l ->
-          eq_args c c' s1 s2 ->
-          P_args c c' s1 s2 ->
-          P_sort c (scon name s1) (scon name s2))
-      (Hsort2 : forall (c : ctx) (t1 t12 t2 : sort),
-          eq_sort c t1 t12 -> P_sort c t1 t12 ->
-          eq_sort c t12 t2 -> P_sort c t12 t2 ->
-          P_sort c t1 t2)
-      (Hsort3 : forall (c : ctx) (t1 t2 : sort),
-          eq_sort c t1 t2 -> P_sort c t1 t2 -> P_sort c t2 t1).
+          eq_args c' s1 s2 ->
+          P_args c' s1 s2 ->
+          P_sort (scon name s1) (scon name s2))
+      (Hsort2 : forall (t1 t12 t2 : sort),
+          eq_sort t1 t12 -> P_sort t1 t12 ->
+          eq_sort t12 t2 -> P_sort t12 t2 ->
+          P_sort t1 t2)
+      (Hsort3 : forall (t1 t2 : sort),
+          eq_sort t1 t2 -> P_sort t1 t2 -> P_sort t2 t1).
     
     (* Term hypotheses *)
-    Context (f : forall (c c' : ctx) (name : V) (t : sort) (e1 e2 : term) s1 s2,
+    Context (f : forall (c' : ctx) (name : V) (t : sort) (e1 e2 : term) s1 s2,
           In (name, term_eq_rule c' e1 e2 t) l ->
-          eq_subst c c' s1 s2 ->
-          P_subst c c' s1 s2 ->
-          P_term c t[/s2/] e1[/s1/] e2[/s2/])
-      (f0 : forall (c c' : ctx) (name : V) (t : sort) args s1 s2,
+          eq_subst c' s1 s2 ->
+          P_subst c' s1 s2 ->
+          P_term t[/s2/] e1[/s1/] e2[/s2/])
+      (f0 : forall (c' : ctx) (name : V) (t : sort) args s1 s2,
           In (name, term_rule c' args t) l ->
-          eq_args c c' s1 s2 ->
-          P_args c c' s1 s2 ->
-          P_term c t[/(with_names_from c' s2)/] (con name s1) (con name s2))
-      (f01 : forall (c : list (V * sort)) (n : V) (t : sort),
-          In (n, t) c -> P_term c t (var n) (var n))
-      (f1 : forall (c : ctx) (t : sort) (e1 e12 e2 : term),
-          eq_term c t e1 e12 -> P_term c t e1 e12 ->
-          eq_term c t e12 e2 -> P_term c t e12 e2 ->
-          P_term c t e1 e2)
-      (f2 : forall (c : ctx) (t : sort) (e1 e2 : term),
-          eq_term c t e1 e2 -> P_term c t e1 e2 -> P_term c t e2 e1)
-      (f3 : forall (c : ctx) (t t' : sort),
-          eq_sort c t t' -> P_sort c t t' ->
+          eq_args c' s1 s2 ->
+          P_args c' s1 s2 ->
+          P_term t[/(with_names_from c' s2)/] (con name s1) (con name s2))
+      (f01 : forall (n : V) (t : sort),
+          In (n, t) c -> P_term t (var n) (var n))
+      (f1 : forall (t : sort) (e1 e12 e2 : term),
+          eq_term t e1 e12 -> P_term t e1 e12 ->
+          eq_term t e12 e2 -> P_term t e12 e2 ->
+          P_term t e1 e2)
+      (f2 : forall (t : sort) (e1 e2 : term),
+          eq_term t e1 e2 -> P_term t e1 e2 -> P_term t e2 e1)
+      (f3 : forall (t t' : sort),
+          eq_sort t t' -> P_sort t t' ->
           forall e1 e2 : term,
-            eq_term c t e1 e2 -> P_term c t e1 e2 -> P_term c t' e1 e2).
+            eq_term t e1 e2 -> P_term t e1 e2 -> P_term t' e1 e2).
 
     (* subst hypotheses *)
-    Context (f4 : forall c : ctx, P_subst c [] [] [])
-      (f5 : forall (c c' : ctx) s1 s2,
-          eq_subst c c' s1 s2 ->
-          P_subst c c' s1 s2 ->
+    Context (f4 : P_subst [] [] [])
+      (f5 : forall (c' : ctx) s1 s2,
+          eq_subst c' s1 s2 ->
+          P_subst c' s1 s2 ->
           forall (name : V) (t : sort) (e1 e2 : term),
-            eq_term c t [/s2/] e1 e2 ->
-            P_term c t [/s2/] e1 e2 ->
-            P_subst c ((name, t) :: c') ((name,e1) :: s1) ((name,e2) :: s2)).
+            eq_term t [/s2/] e1 e2 ->
+            P_term t [/s2/] e1 e2 ->
+            P_subst ((name, t) :: c') ((name,e1) :: s1) ((name,e2) :: s2)).
     
     (* args hypotheses *)
-    Context (f6 : forall c : ctx, P_args c [] [] [])
-      (f7 : forall (c c' : ctx) s1 s2,
-          eq_args c c' s1 s2 ->
-          P_args c c' s1 s2 ->
+    Context (f6 : P_args [] [] [])
+      (f7 : forall (c' : ctx) s1 s2,
+          eq_args c' s1 s2 ->
+          P_args c' s1 s2 ->
           forall (name : V) (t : sort) (e1 e2 : term),
-            eq_term c t [/with_names_from c' s2/] e1 e2 ->
-            P_term c t [/with_names_from c' s2/] e1 e2 ->
-            P_args c ((name, t) :: c') (e1 :: s1) (e2 :: s2)).
+            eq_term t [/with_names_from c' s2/] e1 e2 ->
+            P_term t [/with_names_from c' s2/] e1 e2 ->
+            P_args ((name, t) :: c') (e1 :: s1) (e2 :: s2)).
     
     Section NestedArgs.
-      Context (eq_term_ind' : forall (c : ctx) (s : sort) (t t0 : term),
-                  eq_term c s t t0 -> P_term c s t t0).
-      Arguments eq_term_ind' {_ _ _ _} _.
+      Context (eq_term_ind' : forall (s : sort) (t t0 : term),
+                  eq_term s t t0 -> P_term s t t0).
+      Arguments eq_term_ind' {_ _ _} _.
 
-      Arguments eq_args_cons {c c'}%ctx_scope {es1 es2}%list_scope _
+      Arguments eq_args_cons {c'}%ctx_scope {es1 es2}%list_scope _
         {name t e1 e2} _.
 
-      Arguments f7 {c c'}%ctx_scope {s1 s2}%list_scope _ _ {name t e1 e2} _ _.
+      Arguments f7 {c'}%ctx_scope {s1 s2}%list_scope _ _ {name t e1 e2} _ _.
       
-      Fixpoint eq_args_ind' {c c0 : ctx} {s s0} (e : eq_args c c0 s s0)
-        : P_args c c0 s s0 :=
-        match e in (eq_args c1 c2 s1 s2) return (P_args c1 c2 s1 s2) with
-        | eq_args_nil c1 => f6 c1
+      Fixpoint eq_args_ind' {c0 : ctx} {s s0} (e : eq_args c0 s s0)
+        : P_args c0 s s0 :=
+        match e in (eq_args c2 s1 s2) return (P_args c2 s1 s2) with
+        | eq_args_nil => f6
         | eq_args_cons e0 e3 =>
             f7 e0 (eq_args_ind' e0) e3 (eq_term_ind' e3)
         end.
     End NestedArgs.
     
     Section NestedSubst.
-      Context (eq_term_ind' : forall (c : ctx) (s : sort) (t t0 : term),
-                  eq_term c s t t0 -> P_term c s t t0).
-      Arguments eq_term_ind' {_ _ _ _} _.
+      Context (eq_term_ind' : forall (s : sort) (t t0 : term),
+                  eq_term s t t0 -> P_term s t t0).
+      Arguments eq_term_ind' {_ _ _} _.
 
-      Arguments eq_subst_cons {c c'}%ctx_scope {s1 s2}%list_scope _
+      Arguments eq_subst_cons {c'}%ctx_scope {s1 s2}%list_scope _
         {name t e1 e2} _.
 
-      Arguments f5 {c c'}%ctx_scope {s1 s2}%list_scope _ _ {name t e1 e2} _ _.
+      Arguments f5 {c'}%ctx_scope {s1 s2}%list_scope _ _ {name t e1 e2} _ _.
       
-      Fixpoint eq_subst_ind' {c c0 : ctx} {s s0} (e : eq_subst c c0 s s0)
-        : P_subst c c0 s s0 :=
-        match e in (eq_subst c1 c2 s1 s2) return (P_subst c1 c2 s1 s2) with
-        | eq_subst_nil c1 => f4 c1
+      Fixpoint eq_subst_ind' {c0 : ctx} {s s0} (e : eq_subst c0 s s0)
+        : P_subst c0 s s0 :=
+        match e in (eq_subst c2 s1 s2) return (P_subst c2 s1 s2) with
+        | eq_subst_nil => f4
         | eq_subst_cons e0 e3 =>
             f5 e0 (eq_subst_ind' e0) e3 (eq_term_ind' e3)
         end.
     End NestedSubst.
 
-    Fixpoint eq_sort_ind' [c t t0]
-      (e : eq_sort c t t0) : P_sort c t t0 :=
-           match e in (eq_sort c0 t1 t2) return (P_sort c0 t1 t2) with
-           | eq_sort_by c0 name c' e1 e2 s1 s2 i pa =>
-               Hsort0 c0 c' name e1 e2 s1 s2 i pa (eq_subst_ind' eq_term_ind' pa)
-           | eq_sort_cong c0 name c' args s1 s2 i pa =>
-               Hsort1 c0 c' name args s1 s2 i pa (eq_args_ind' eq_term_ind' pa)
-           | eq_sort_trans _ _ _ _ e0 e3 =>
-               Hsort2 _ _ _ _ e0 (eq_sort_ind' e0) e3 (eq_sort_ind' e3)
-           | eq_sort_sym _ _ _ e0 => Hsort3 _ _ _ e0 (eq_sort_ind' e0)
+    Fixpoint eq_sort_ind' [t t0]
+      (e : eq_sort t t0) : P_sort t t0 :=
+           match e in (eq_sort t1 t2) return (P_sort t1 t2) with
+           | eq_sort_by name c' e1 e2 s1 s2 i pa =>
+               Hsort0 c' name e1 e2 s1 s2 i pa (eq_subst_ind' eq_term_ind' pa)
+           | eq_sort_cong name c' args s1 s2 i pa =>
+               Hsort1 c' name args s1 s2 i pa (eq_args_ind' eq_term_ind' pa)
+           | eq_sort_trans _ _ _ e0 e3 =>
+               Hsort2 _ _ _ e0 (eq_sort_ind' e0) e3 (eq_sort_ind' e3)
+           | eq_sort_sym _ _ e0 => Hsort3 _ _ e0 (eq_sort_ind' e0)
            end
-    with eq_term_ind' [c s t t0]
-      (e : eq_term c s t t0) : P_term c s t t0 :=
-           match e in (eq_term c0 s0 t1 t2) return (P_term c0 s0 t1 t2) with
-           | eq_term_by c0 name c' t1 e1 e2 s1 s2 i pa =>
-               f c0 c' name t1 e1 e2 s1 s2 i pa (eq_subst_ind' eq_term_ind' pa)
-           | eq_term_cong c0 name c' args t1 s1 s2 i pa =>
-               f0 c0 c' name t1 args s1 s2 i pa (eq_args_ind' eq_term_ind' pa)
-           | eq_term_var c0 n t0 i => f01 c0 n t0 i
-           | eq_term_trans _ _ _ _ _ e0 e3 =>
-               f1 _ _ _ _ _ e0 (eq_term_ind' e0) e3 (eq_term_ind' e3)
-           | eq_term_sym _ _ _ _ e0 => f2 _ _ _ _ e0 (eq_term_ind' e0)
-           | eq_term_conv _ _ _ _ _ e3 e0 =>
-               f3 _ _ _ e0 (eq_sort_ind' e0) _ _ e3 (eq_term_ind' e3)
+    with eq_term_ind' [s t t0]
+      (e : eq_term s t t0) : P_term s t t0 :=
+           match e in (eq_term s0 t1 t2) return (P_term s0 t1 t2) with
+           | eq_term_by name c' t1 e1 e2 s1 s2 i pa =>
+               f c' name t1 e1 e2 s1 s2 i pa (eq_subst_ind' eq_term_ind' pa)
+           | eq_term_cong name c' args t1 s1 s2 i pa =>
+               f0 c' name t1 args s1 s2 i pa (eq_args_ind' eq_term_ind' pa)
+           | eq_term_var n t0 i => f01 n t0 i
+           | eq_term_trans _ _ _ _ e0 e3 =>
+               f1 _ _ _ _ e0 (eq_term_ind' e0) e3 (eq_term_ind' e3)
+           | eq_term_sym _ _ _ e0 => f2 _ _ _ e0 (eq_term_ind' e0)
+           | eq_term_conv _ _ _ _ e3 e0 =>
+               f3 _ _ e0 (eq_sort_ind' e0) _ _ e3 (eq_term_ind' e3)
            end.
     
     Definition eq_args_ind'' := @eq_args_ind' eq_term_ind'.
@@ -305,45 +381,260 @@ c |- e1 = e2 : t'
               eq_args_ind'')).
   End EqInd.
 
-  Context (wfl : wf_lang l).
   
-  Local Lemma cut_implies_core 
-    : (forall c t1 t2,
-          eq_sort c t1 t2 ->
-          Core.eq_sort l c t1 t2)
-      /\ (forall c t e1 e2,
-             eq_term c t e1 e2 ->
-             Core.eq_term l c t e1 e2)
-      /\ (forall c c' s1 s2,
-             eq_subst c c' s1 s2 ->
-             Model.eq_subst (Model := core_model l) c c' s1 s2)
-      /\ (forall c c' s1 s2,
-             eq_args c c' s1 s2 ->
-             Model.eq_args (Model := core_model l) c c' s1 s2).
-  Proof using V_Eqb_ok wfl.
+  Local Hint Constructors eq_sort eq_term eq_subst eq_args : lang_core.
+  
+  Local Lemma eq_refl_right
+    : (forall t1 t2,
+          eq_sort t1 t2 ->
+          eq_sort t2 t2)
+      /\ (forall t e1 e2,
+             eq_term t e1 e2 ->
+             eq_term t e2 e2)
+      /\ (forall c' s1 s2,
+             eq_subst c' s1 s2 ->
+             eq_subst c' s2 s2)
+      /\ (forall c' s1 s2,
+             eq_args c' s1 s2 ->
+             eq_args c' s2 s2).
+  Proof using V_Eqb_ok.
     simple eapply cut_ind;
       basic_goal_prep;
       basic_core_crush.
-    all: eauto using
-           sort_con_congruence,
-        Core.eq_sort_trans, Core.eq_sort_sym,
-        term_con_congruence,
-        Core.eq_term_trans, Core.eq_term_sym.
   Qed.
-
-  Definition eq_sort_cut_implies_core := proj1 cut_implies_core.
-  Local Hint Resolve eq_sort_cut_implies_core : lang_core.
+        
+  Definition eq_sort_refl_right := proj1 eq_refl_right.
+  Local Hint Resolve eq_sort_refl_right : lang_core.
   
-  Definition eq_term_cut_implies_core := proj1 (proj2 cut_implies_core).
-  Local Hint Resolve eq_term_cut_implies_core : lang_core.
+  Definition eq_term_refl_right := proj1 (proj2 eq_refl_right).
+  Local Hint Resolve eq_term_refl_right : lang_core.
 
-  Definition eq_subst_cut_implies_core := proj1 (proj2 (proj2 cut_implies_core)).
-  Local Hint Resolve eq_subst_cut_implies_core : lang_core.
+  Definition eq_subst_refl_right := proj1 (proj2 (proj2 eq_refl_right)).
+  Local Hint Resolve eq_subst_refl_right : lang_core.
   
-  Definition eq_args_cut_implies_core := proj2 (proj2 (proj2 cut_implies_core)).
-  Local Hint Resolve eq_args_cut_implies_core : lang_core.
+  Definition eq_args_refl_right := proj2 (proj2 (proj2 eq_refl_right)).
+  Local Hint Resolve eq_args_refl_right : lang_core.
+
+  
+  Lemma eq_args_implies_eq_subst:
+  forall [c' : NamedList.named_list V sort] [s1 s2 : list term],
+    eq_args c' s1 s2 -> eq_subst c' (with_names_from c' s1) (with_names_from c' s2).
+  Proof.
+    induction 1;
+      basic_goal_prep;
+      basic_core_crush.
+  Qed.
+  Hint Resolve eq_args_implies_eq_subst : lang_core.
+
+  
+  Lemma eq_subst_map_fst_r c0 s0 s3
+    : eq_subst c0 s0 s3 -> map fst s3 = map fst c0.
+  Proof.
+    induction 1;
+      basic_goal_prep;
+      basic_core_crush.
+  Qed.
+  #[local] Hint Rewrite eq_subst_map_fst_r using eassumption : lang_core.
+
+  Lemma eq_subst_map_fst_l c0 s0 s3
+    : eq_subst c0 s0 s3 -> map fst s0 = map fst c0.
+  Proof.
+    induction 1;
+      basic_goal_prep;
+      basic_core_crush.
+  Qed.
+  #[local] Hint Rewrite eq_subst_map_fst_l using eassumption : lang_core.
+
+
+  Lemma eq_subst_fresh_r c0 s0 s3 n
+    : eq_subst c0 s0 s3 -> fresh n c0 -> fresh n s3.
+  Proof.
+    unfold fresh; intros.
+    erewrite eq_subst_map_fst_r; eauto.
+  Qed.
+  #[local] Hint Resolve eq_subst_fresh_r : lang_core.
+
+  Lemma eq_subst_fresh_l c0 s0 s3 n
+    : eq_subst c0 s0 s3 -> fresh n c0 -> fresh n s0.
+  Proof.
+    unfold fresh; intros.
+    erewrite eq_subst_map_fst_l; eauto.
+  Qed.
+  #[local] Hint Resolve eq_subst_fresh_l : lang_core.
+
+  
+  
+  Lemma eq_args_len_eq_r c' s1 s2
+    : eq_args c' s1 s2 ->
+      length s2 = length c'.
+  Proof.
+    induction 1; basic_goal_prep;
+      basic_core_crush.
+  Qed.
+  (*Hint Rewrite eq_args_len_eq_r using eassumption : lang_core.*)
+  
+  
+  Lemma eq_args_len_eq_l c' s1 s2
+    : eq_args c' s1 s2 ->
+      length s1 = length c'.
+  Proof.
+    induction 1; basic_goal_prep;
+      basic_core_crush.
+  Qed.
+  (*Hint Rewrite eq_args_len_eq_l using eassumption : lang_core.*)
+  
+  Section __.
+    Context (wsl : ws_lang l)
+      (wsc : ws_ctx c).
+    
+    Lemma eq_implies_ws
+      : (forall t1' t2',
+            eq_sort t1' t2' ->
+            well_scoped (map fst c) t1'
+            /\ well_scoped (map fst c) t2')
+        /\ (forall (t : Term.sort V) (e1 e2 : Term.term V),
+               eq_term t e1 e2 ->
+               well_scoped (map fst c) t
+               /\ well_scoped (map fst c) e1
+               /\ well_scoped (map fst c) e2)
+        /\ (forall (c' : Term.ctx V) (s1 s2 : Term.subst V),
+              eq_subst c' s1 s2 ->
+              ws_ctx c' ->
+              well_scoped (map fst c) s1
+              /\ well_scoped (map fst c) s2)
+        /\ (forall c' (s1 s2 : list term),
+               eq_args c' s1 s2 ->
+               ws_ctx c' ->
+               well_scoped (map fst c) s1
+               /\ well_scoped (map fst c) s2).
+    Proof using V_Eqb_ok wsl wsc.
+      simple eapply cut_ind;
+        basic_goal_prep.
+      all: try use_rule_in_ws.
+      all: basic_goal_prep.
+      all: autorewrite with utils model term lang_core in *.
+      all: basic_goal_prep.
+      all: intuition subst.
+      all: try eapply well_scoped_subst; eauto; try typeclasses eauto.
+      all: eauto with utils model term lang_core.
+      all: try change (ws_subst ?a ?b) with (well_scoped a b).
+      all: try change (ws_args ?a ?b) with (well_scoped a b).
+      all: try erewrite eq_subst_map_fst_l by eassumption; eauto.
+      all: try erewrite eq_subst_map_fst_r by eassumption; eauto.
+      all: try eapply ws_subst_from_ws_args.
+      all: try eauto using ws_all_fresh_ctx.
+      all: try erewrite eq_args_len_eq_r; eauto.
+      basic_utils_crush.
+      erewrite eq_args_len_eq_r; eauto.
+    Qed.
+
+    Definition eq_sort_implies_ws_l t1' t2' (Heq : eq_sort t1' t2') :=
+      proj1 ((proj1 eq_implies_ws) _ _ Heq).
+    Definition eq_sort_implies_ws_r t1' t2' (Heq : eq_sort t1' t2') :=
+      proj2 ((proj1 eq_implies_ws) _ _ Heq).
+    Definition eq_term_implies_ws_sort t e1 e2 (Heq : eq_term t e1 e2) :=
+      proj1 ((proj1 (proj2 eq_implies_ws)) _ _ _ Heq).
+    Definition eq_term_implies_ws_l t e1 e2 (Heq : eq_term t e1 e2) :=
+      proj1 (proj2 ((proj1 (proj2 eq_implies_ws)) _ _ _ Heq)).
+    Definition eq_term_implies_ws_r t e1 e2 (Heq : eq_term t e1 e2) :=
+      proj2 (proj2 ((proj1 (proj2 eq_implies_ws)) _ _ _ Heq)).
+    Definition eq_subst_implies_ws_l c' s1 s2 (Heq : eq_subst c' s1 s2) Hws' :=
+      proj1 ((proj1 (proj2 (proj2 eq_implies_ws))) _ _ _ Heq Hws').
+    Definition eq_subst_implies_ws_r c' s1 s2 (Heq : eq_subst c' s1 s2) Hws' :=
+      proj2 ((proj1 (proj2 (proj2 eq_implies_ws))) _ _ _ Heq Hws').
+    Definition eq_args_implies_ws_l c' s1 s2 (Heq : eq_args c' s1 s2) Hws' :=
+      proj1 ((proj2 (proj2 (proj2 eq_implies_ws))) _ _ _ Heq Hws').
+    Definition eq_args_implies_ws_r c' s1 s2 (Heq : eq_args c' s1 s2) Hws' :=
+      proj2 ((proj2 (proj2 (proj2 eq_implies_ws))) _ _ _ Heq Hws').
+    
+    Hint Resolve eq_sort_implies_ws_l : lang_core.
+    Hint Resolve eq_sort_implies_ws_r : lang_core.
+    Hint Resolve eq_term_implies_ws_sort : lang_core. 
+    Hint Resolve eq_term_implies_ws_l : lang_core. 
+    Hint Resolve eq_term_implies_ws_r : lang_core.  
+    Hint Resolve eq_subst_implies_ws_l : lang_core.
+    Hint Resolve eq_subst_implies_ws_r : lang_core.
+    Hint Resolve eq_args_implies_ws_l : lang_core.
+    Hint Resolve eq_args_implies_ws_r : lang_core.
+
+  End __.
+  
+  
+  End WithCtx.
 
   Local Hint Constructors eq_sort eq_term eq_subst eq_args : lang_core.
+  Local Hint Resolve eq_sort_refl_right : lang_core.
+  Local Hint Resolve eq_term_refl_right : lang_core.
+  Local Hint Resolve eq_subst_refl_right : lang_core.
+  Local Hint Resolve eq_args_refl_right : lang_core.
+  Hint Resolve eq_args_implies_eq_subst : lang_core.
+
+  #[local] Hint Rewrite eq_subst_map_fst_r using eassumption : lang_core.
+  #[local] Hint Rewrite eq_subst_map_fst_l using eassumption : lang_core.
+  #[local] Hint Resolve eq_subst_fresh_r : lang_core.
+  #[local] Hint Resolve eq_subst_fresh_l : lang_core.
+
+  
+  Hint Resolve eq_sort_implies_ws_l : lang_core.
+  Hint Resolve eq_sort_implies_ws_r : lang_core.
+  Hint Resolve eq_term_implies_ws_sort : lang_core. 
+  Hint Resolve eq_term_implies_ws_l : lang_core. 
+  Hint Resolve eq_term_implies_ws_r : lang_core.  
+  Hint Resolve eq_subst_implies_ws_l : lang_core.
+  Hint Resolve eq_subst_implies_ws_r : lang_core.
+  Hint Resolve eq_args_implies_ws_l : lang_core.
+  Hint Resolve eq_args_implies_ws_r : lang_core.
+
+  
+
+  Inductive wf_ctx : named_list sort -> Prop :=
+    wf_ctx_nil : wf_ctx []
+  | wf_ctx_cons : forall name c t,
+      fresh name c -> wf_ctx c -> eq_sort c t t -> wf_ctx ((name, t) :: c).
+  Hint Constructors wf_ctx : lang_core.
+
+  
+  Lemma invert_wf_ctx_nil : wf_ctx [] <-> True.
+  Proof. solve_invert_constr_eq_lemma. Qed.
+  #[local] Hint Rewrite invert_wf_ctx_nil : lang_core.
+
+  Lemma invert_wf_ctx_cons c n t
+    : wf_ctx ((n,t)::c) <-> fresh n c /\ wf_ctx c /\ eq_sort c t t.
+  Proof. solve_invert_constr_eq_lemma. Qed.
+  #[local] Hint Rewrite invert_wf_ctx_cons : lang_core.
+
+  
+  Local Lemma ctx_mono c c'
+    : incl c c' ->
+      (forall t1 t2,
+          eq_sort c t1 t2 ->
+          eq_sort c' t1 t2)
+      /\ (forall t e1 e2,
+             eq_term c t e1 e2 ->
+             eq_term c' t e1 e2)
+      /\ (forall c'' s1 s2,
+             eq_subst c c'' s1 s2 ->
+             eq_subst c' c'' s1 s2)
+      /\ (forall c'' s1 s2,
+             eq_args c c'' s1 s2 ->
+             eq_args c' c'' s1 s2).
+  Proof using V_Eqb_ok.
+    intro Hincl.
+    eapply cut_ind;
+      basic_goal_prep;
+      basic_core_crush.
+  Qed.
+
+  Lemma in_ctx_wf n t c
+    : wf_ctx c -> In (n, t) c -> eq_sort c t t.
+  Proof.
+    induction 1;
+      basic_goal_prep;
+      basic_core_crush.
+    all:eapply ctx_mono; eauto; eauto with utils.
+  Qed.
+  Hint Resolve in_ctx_wf : lang_core.
+
 
   Lemma cut_id_subst_refl' c c'
     : incl c c' -> eq_subst c' c (id_subst c) (id_subst c).
@@ -366,134 +657,6 @@ c |- e1 = e2 : t'
     eapply cut_id_subst_refl'; basic_utils_crush.
   Qed.
   Hint Resolve cut_id_subst_refl : lang_core.
-
-  Local Lemma eq_refl_right
-    : (forall c t1 t2,
-          eq_sort c t1 t2 ->
-          eq_sort c t2 t2)
-      /\ (forall c t e1 e2,
-             eq_term c t e1 e2 ->
-             eq_term c t e2 e2)
-      /\ (forall c c' s1 s2,
-             eq_subst c c' s1 s2 ->
-             eq_subst c c' s2 s2)
-      /\ (forall c c' s1 s2,
-             eq_args c c' s1 s2 ->
-             eq_args c c' s2 s2).
-  Proof using V_Eqb_ok wfl.
-    simple eapply cut_ind;
-      basic_goal_prep;
-      basic_core_crush.
-    all: eauto using
-           sort_con_congruence,
-        Core.eq_sort_trans, Core.eq_sort_sym,
-        term_con_congruence,
-        Core.eq_term_trans, Core.eq_term_sym.
-  Qed.
-        
-  Definition eq_sort_refl_right := proj1 eq_refl_right.
-  Local Hint Resolve eq_sort_refl_right : lang_core.
-  
-  Definition eq_term_refl_right := proj1 (proj2 eq_refl_right).
-  Local Hint Resolve eq_term_refl_right : lang_core.
-
-  Definition eq_subst_refl_right := proj1 (proj2 (proj2 eq_refl_right)).
-  Local Hint Resolve eq_subst_refl_right : lang_core.
-  
-  Definition eq_args_refl_right := proj2 (proj2 (proj2 eq_refl_right)).
-  Local Hint Resolve eq_args_refl_right : lang_core.
-
-  (*TODO: Do I need wfness for admissibility?*)
-  Notation wf_ctx :=
-    (wf_ctx (Model:= core_model l)).
-
-  Lemma eq_args_implies_eq_subst:
-  forall [c c' : NamedList.named_list V sort] [s1 s2 : list term],
-    eq_args c c' s1 s2 -> eq_subst c c' (with_names_from c' s1) (with_names_from c' s2).
-  Proof.
-    induction 1;
-      basic_goal_prep;
-      basic_core_crush.
-  Qed.
-  Hint Resolve eq_args_implies_eq_subst : lang_core.
-
-  
-  
-(*
-  Lemma cut_admissible1
-    : (forall c' t1' t2',
-          eq_sort c' t1' t2' ->
-          forall c s,
-            eq_subst c c' s s ->
-            wf_ctx c' ->
-            eq_sort c t1' [/s/] t2' [/s/])
-      /\ (forall c' (t : Term.sort V) (e1 e2 : Term.term V),
-             eq_term c' t e1 e2 ->
-             forall c s,
-             eq_subst c c' s s ->
-             wf_ctx c' -> eq_term c t [/s/] e1 [/s/] e2 [/s/])
-      /\ ((*wf_lang l ->*)
-          forall (c c' : Term.ctx V) (s1 s2 : Term.subst V),
-            eq_subst c c' s1 s2 ->
-            wf_ctx c ->
-            wf_ctx c' ->
-            forall (c'' : Term.ctx V) (s' : Term.subst V),
-              eq_subst c'' c s' s' ->
-              eq_subst c'' c' s1 [/s' /] s2 [/s' /])
-      /\ (forall c c' (s1 s2 : list term),
-            eq_args c c' s1 s2 ->
-            wf_ctx c ->
-            wf_ctx c' ->
-            forall c'' s',
-              eq_subst c'' c s' s' ->
-              eq_args c'' c' s1 [/s'/] s2 [/s'/]).
-  Proof.
-    simple eapply cut_ind.
-    all: basic_goal_prep.
-    all: erewrite ?subst_assoc; try typeclasses eauto;[|shelve..].
-    all: fold_Substable.
-    all: basic_core_crush.
-    {
-      rewrite <- !Substable.with_names_from_args_subst.
-      eapply eq_term_cong; eauto.
-      eapply H4; eauto.
-      basic_core_crush.
-    }
-    {
-      admit (*TODO: var lemma*).
-    }
-    {
-      constructor; eauto.
-      unfold apply_subst at 2; cbn [substable_subst].
-      erewrite <- subst_assoc; eauto.
-      1: typeclasses eauto.
-      basic_core_crush.
-    }
-    {
-      constructor; eauto.
-      rewrite !Substable.with_names_from_args_subst.
-      unfold apply_subst at 2; cbn [substable_subst].
-      erewrite <- subst_assoc; eauto.
-      1: typeclasses eauto.
-      basic_core_crush.
-    }
-    Unshelve.
-    all: basic_core_crush.
-    {
-      replace (map fst s2) with (map fst c') by admit (*TODO: lemma*).
-      use_rule_in_wf.
-      autorewrite with utils lang_core in *.
-      break.
-      eauto with lang_core.
-    }
-    {
-      use_rule_in_wf.      
-      autorewrite with utils lang_core in *.
-      break.
-      eauto with lang_core.
-    }
-  Admitted.
- *)
 
   Definition sort_cut_admissible c' t1' t2' :=
     forall c s1 s2,
@@ -560,87 +723,7 @@ c |- e1 = e2 : t'
         ctx_cut_admissible c
         /\ sort_cut_admissible c t t
     end.
-
-  (*Note: proof of this depends on weakening*)
-  Context (lang_admissible : all rule_cut_admissible (map snd l)).
-
-  (*TODO: can I generalize the above to a kind of induction scheme?
-    TODO: generic over language too?
-
-    Record is a distraction.
-    What I want: judge_ind, but nested w/ an induction over the language.
-    Doesn't seem like there's much in the way of simplification to be gained right now.
-
-  Record PyrosomeProperty : Prop :=
-    {|
-      P_eq_sort : lang -> Term.ctx V -> Term.sort V -> Term.sort V -> Prop;
-      P_eq_term : lang -> Term.ctx V -> Term.sort V -> Term.term V -> Term.term V -> Prop;
-      (* commented properties should be derivable? Maybe no...*)
-      (*P_eq_subst : lang -> Term.ctx V -> Term.ctx V -> Term.subst V -> Term.subst V -> Prop;*)
-      P_wf_sort : lang -> Term.ctx V -> Term.sort V -> Prop; (*TODO: could just make this refl?*)
-      P_wf_term : lang -> Term.ctx V -> Term.term V -> Term.sort V -> Prop;
-      (*P_wf_args : lang -> Term.ctx V -> list (Term.term V) -> Term.ctx V -> Prop;*)
-      (*P_wf_ctx : lang -> Term.ctx V -> Prop;*)
-      (*P_wf_rule : lang -> rule -> Prop;*)
-      (*P_wf_lang : lang -> Term.ctx V -> Prop;*)
-    |}.
-   *)
-  (*
-  Section Nested.
-    Context (core_implies_cut
-    : (forall c t1 t2,
-          Core.eq_sort l c t1 t2 ->
-          ctx_all_admissible c ->
-          eq_sort c t1 t2)
-      /\ (forall c t e1 e2,
-             Core.eq_term l c t e1 e2 ->
-             ctx_all_admissible c ->
-             eq_term c t e1 e2)
-      /\ (forall c c' s1 s2,
-             Model.eq_subst (Model:= core_model l) c c' s1 s2 ->
-             ctx_all_admissible c ->
-             eq_subst c c' s1 s2)
-      /\ (forall c t,
-             wf_sort l c t ->
-             eq_sort c t t)
-      /\ (forall c e t,
-             wf_term l c e t ->
-             eq_term c t e e)
-      /\ (forall c s c',
-             wf_args (Model:= core_model l) c s c' ->
-             eq_args c c' s s)
-      /\ (forall c,
-             Model.wf_ctx (Model:= core_model l) c -> ctx_all_admissible c)).
-
-    Context (cut_admissible
-    : (forall c' t1' t2',
-          eq_sort c' t1' t2' ->
-          forall c s1 s2,
-            eq_subst c c' s1 s2 ->
-            wf_ctx c' ->
-            eq_sort c t1' [/s1 /] t2' [/s2 /])
-      /\ (forall c' (t : Term.sort V) (e1 e2 : Term.term V),
-             eq_term c' t e1 e2 ->
-             forall c s1 s2,
-             eq_subst c c' s1 s2 ->
-             wf_ctx c' -> eq_term c t [/s2 /] e1 [/s1 /] e2 [/s2 /])
-      /\ ((*wf_lang l ->*)
-          forall (c c' : Term.ctx V) (s1 s2 : Term.subst V),
-            eq_subst c c' s1 s2 ->
-            wf_ctx c ->
-            wf_ctx c' ->
-            forall (c'' : Term.ctx V) (s1' s2' : Term.subst V),
-              eq_subst c'' c s1' s2' ->
-              eq_subst c'' c' s1 [/s1' /] s2 [/s2' /])
-      /\ (forall c c' (s1 s2 : list term),
-            eq_args c c' s1 s2 ->
-            wf_ctx c ->
-            wf_ctx c' ->
-            forall c'' s1' s2',
-              eq_subst c'' c s1' s2' ->
-              eq_args c'' c' s1 [/s1' /] s2 [/s2' /])).
-   *)
-
+  
   Lemma eq_subst_sym' c c' s1 s2
     : eq_subst c c' s1 s2 -> wf_ctx c' -> ctx_cut_admissible c' -> eq_subst c c' s2 s1.
   Proof using .
@@ -656,129 +739,335 @@ c |- e1 = e2 : t'
     eapply H2; eauto.
   Qed.
 
-  Lemma refl_term_lookup c0 c s1 s2 n t
-    : eq_subst c0 c s1 s2 ->
+
+  Variant wf_rule : rule -> Prop :=
+  | wf_sort_rule : forall c args,
       wf_ctx c ->
-      In (n, t) c ->
-      eq_term c0 t [/s2 /] (term_subst_lookup s1 n) (term_subst_lookup s2 n).
+      sublist args (map fst c) ->
+      wf_rule (sort_rule c args)
+  | wf_term_rule : forall c args t,
+      wf_ctx c ->
+      eq_sort c t t ->
+      sublist args (map fst c) ->
+      wf_rule (term_rule c args t)
+  | eq_sort_rule : forall c t1 t2,
+      wf_ctx c ->
+      eq_sort c t1 t1 ->
+      eq_sort c t2 t2 ->
+      wf_rule (sort_eq_rule c t1 t2)
+  | eq_term_rule : forall c e1 e2 t,
+      wf_ctx c ->
+      eq_sort c t t ->
+      eq_term c t e1 e1 ->
+      eq_term c t e2 e2 ->
+      wf_rule (term_eq_rule c e1 e2 t).
+
+  
+  Lemma invert_wf_sort_rule c args
+    : wf_rule (sort_rule c args) <-> wf_ctx c /\ sublist args (map fst c).
+  Proof. solve_invert_constr_eq_lemma. Qed.
+  Hint Rewrite invert_wf_sort_rule : lang_core.
+
+  Lemma invert_wf_term_rule c args t
+    : wf_rule (term_rule c args t) <-> wf_ctx c /\ sublist args (map fst c) /\ eq_sort c t t.
+  Proof. solve_invert_constr_eq_lemma. Qed.
+  Hint Rewrite invert_wf_term_rule : lang_core.
+
+  Lemma invert_wf_sort_eq_rule c t1 t2
+    : wf_rule (sort_eq_rule c t1 t2) <-> wf_ctx c /\ eq_sort c t1 t1 /\ eq_sort c t2 t2.
+  Proof. solve_invert_constr_eq_lemma. Qed.
+  Hint Rewrite invert_wf_sort_eq_rule : lang_core.
+
+  Lemma invert_wf_term_eq_rule c e1 e2 t
+    : wf_rule (term_eq_rule c e1 e2 t)
+      <-> wf_ctx c /\ eq_term c t e1 e1 /\ eq_term c t e2 e2 /\ eq_sort c t t.
+  Proof. solve_invert_constr_eq_lemma. Qed.
+  Hint Rewrite invert_wf_term_eq_rule : lang_core.
+
+
+
+  Section __.
+    Context (wsl : ws_lang l).
+
+    Lemma wf_ctx_implies_ws c
+      : wf_ctx c -> ws_ctx c.
+    Proof.
+      induction 1;
+        basic_goal_prep;
+        basic_core_crush.
+      eapply eq_sort_implies_ws_l; eauto.
+    Qed.
+    Hint Resolve wf_ctx_implies_ws : lang_core.
+
+    
+    Lemma wf_rule_implies_ws r
+      : wf_rule r -> ws_rule r.
+    Proof.
+      destruct 1;
+        basic_goal_prep;
+        autorewrite with utils term lang_core in *;
+        intuition eauto with lang_core.
+    Qed.
+
+    
+    Lemma ctx_admissible_in c n t
+      : wf_ctx c ->
+        ctx_cut_admissible c ->
+        In (n, t) c ->
+        sort_cut_admissible c t t.
+    Proof using V_Eqb_ok wsl.
+      induction 1;
+        basic_goal_prep;
+        basic_core_crush.
+      {
+        clear H3.
+        unfold sort_cut_admissible in *;
+          intros.
+        safe_invert H2.
+        safe_invert H3.
+        erewrite !strengthen_subst;
+          try typeclasses eauto;
+          eauto.
+        all: try erewrite eq_subst_map_fst_l by eassumption; eauto.
+        all: try erewrite eq_subst_map_fst_r by eassumption; eauto.
+        all: try (eapply eq_subst_fresh_l; now eauto).
+        all: try (eapply eq_subst_fresh_r; now eauto).
+        all: eapply eq_sort_implies_ws_r; eauto with lang_core.
+      }
+      {
+        clear H4.      
+        unfold sort_cut_admissible in *;
+          intros.
+        safe_invert H3.
+        eapply in_ctx_wf in H2; eauto.
+        erewrite !strengthen_subst;
+          try typeclasses eauto;
+          eauto.
+        2,4:basic_core_crush.
+        all: try erewrite eq_subst_map_fst_l by eassumption; eauto.
+        all: try erewrite eq_subst_map_fst_r by eassumption; eauto.
+        all: eauto with lang_core.
+      }
+    Qed.
+
+    
+    
+    Lemma refl_term_lookup c0 c s1 s2 n t
+      : eq_subst c0 c s1 s2 ->
+        wf_ctx c ->
+        In (n, t) c ->
+        eq_term c0 t [/s2 /] (term_subst_lookup s1 n) (term_subst_lookup s2 n).
+    Proof.
+      induction 1;
+        basic_goal_prep;
+        autorewrite with utils term lang_core model in *;
+        [tauto|].
+      intuition subst.
+      {
+        rewrite strengthen_subst with (Substable0 := _);
+          try typeclasses eauto.
+        all: try erewrite eq_subst_map_fst_r by eassumption; eauto.
+        all:basic_core_crush.        
+      }
+      {
+        cbn.
+        case_match; basic_goal_prep; autorewrite with utils term lang_core model in *;
+          subst.
+        {
+          erewrite strengthen_subst;
+            try typeclasses eauto;
+            eauto;
+            basic_core_crush.
+        }
+        {
+          change ((named_list_lookup (var ?n) ?s ?n)) with (subst_lookup s n).
+          erewrite strengthen_subst;
+            try typeclasses eauto;
+            eauto.
+          all: try erewrite eq_subst_map_fst_r by eassumption; eauto.
+          all: basic_core_crush.
+        }
+      }
+    Qed.
+    Hint Resolve refl_term_lookup : lang_core.
+
+  End __.
+
+  (*
+  (*Note: proof of this depends on weakening*)
+  Context (lang_admissible : all rule_cut_admissible (map snd l)).
+   *)
+
+End Terms.
+
+Hint Resolve eq_sort_by eq_term_by eq_sort_cong eq_term_cong : lang_core.
+Hint Constructors eq_subst eq_args : lang_core.
+
+Hint Resolve eq_sort_implies_ws_l : lang_core.
+Hint Resolve eq_sort_implies_ws_r : lang_core.
+Hint Resolve eq_term_implies_ws_sort : lang_core. 
+Hint Resolve eq_term_implies_ws_l : lang_core. 
+Hint Resolve eq_term_implies_ws_r : lang_core.  
+Hint Resolve eq_subst_implies_ws_l : lang_core.
+Hint Resolve eq_subst_implies_ws_r : lang_core.
+Hint Resolve eq_args_implies_ws_l : lang_core.
+Hint Resolve eq_args_implies_ws_r : lang_core.
+Hint Resolve wf_ctx_implies_ws : lang_core.
+Hint Resolve wf_rule_implies_ws : lang_core.
+
+
+Hint Resolve refl_term_lookup : lang_core.
+
+Hint Constructors wf_ctx wf_rule : lang_core.
+
+Hint Rewrite invert_wf_ctx_nil : lang_core.
+Hint Rewrite invert_wf_ctx_cons : lang_core.
+
+Hint Rewrite invert_wf_sort_rule : lang_core.
+Hint Rewrite invert_wf_term_rule : lang_core.
+Hint Rewrite invert_wf_sort_eq_rule : lang_core.
+Hint Rewrite invert_wf_term_eq_rule : lang_core.
+
+
+Section LangMono.
+  Context (l l': lang).
+  Context (Hincl : incl l l').
+
+  Section __.
+    Context (c : ctx).
+    Local Lemma lang_mono 
+      : (forall t1 t2,
+            eq_sort l c t1 t2 ->
+            eq_sort l' c t1 t2)
+        /\ (forall t e1 e2,
+               eq_term l c t e1 e2 ->
+               eq_term l' c t e1 e2)
+        /\ (forall c' s1 s2,
+               eq_subst l c c' s1 s2 ->
+               eq_subst l' c c' s1 s2)
+        /\ (forall c' s1 s2,
+               eq_args l c c' s1 s2 ->
+               eq_args l' c c' s1 s2).
+    Proof using Hincl c.
+      eapply cut_ind;
+        basic_goal_prep;
+        try solve [constructor; eauto].
+      { eapply eq_sort_by; eauto. }
+      { eapply eq_sort_cong; eauto. }
+      { eapply eq_sort_trans; eauto. }
+      { eapply eq_term_by; eauto. }
+      { eapply eq_term_cong; eauto. }
+      { eapply eq_term_trans; eauto. }
+      { eapply eq_term_conv; eauto. }
+    Qed.
+
+    Definition eq_sort_lang_mono := proj1 lang_mono.
+    Definition eq_term_lang_mono := proj1 (proj2 lang_mono).
+    Definition eq_subst_lang_mono := proj1 (proj2 (proj2 lang_mono)).
+    Definition eq_args_lang_mono := proj2 (proj2 (proj2 lang_mono)).
+    
+  End __.
+
+  Hint Resolve eq_sort_lang_mono : lang_core.
+  Hint Resolve eq_term_lang_mono : lang_core.
+  
+  Lemma ctx_lang_mono c
+    : wf_ctx l c -> wf_ctx l' c.
   Proof.
     induction 1;
       basic_goal_prep;
       basic_core_crush.
-  {
-    rewrite strengthen_subst with (Substable0 := _);
-    try typeclasses eauto;
-      basic_core_crush.
-  }
-  {
-    cbn.
-    case_match; basic_goal_prep; autorewrite with utils term lang_core model in *;
-      subst.
-    {
-      erewrite strengthen_subst;
-        try typeclasses eauto;
-        eauto;
-        basic_core_crush.
-    }
-    {
-      change ((named_list_lookup (var ?n) ?s ?n)) with (subst_lookup s n).
-      erewrite strengthen_subst;
-        try typeclasses eauto;
-        eauto;
-        basic_core_crush.
-    }
-  }
-Qed.
-Hint Resolve refl_term_lookup : lang_core.  
-
-
-Lemma eq_subst_map_fst_r c0 c s0 s3
-  : eq_subst c0 c s0 s3 -> map fst s3 = map fst c.
-Proof.
-  induction 1;
-    basic_goal_prep;
-    basic_core_crush.
-Qed.
-#[local] Hint Rewrite eq_subst_map_fst_r using eassumption : lang_core.
-
-Lemma eq_subst_map_fst_l c0 c s0 s3
-  : eq_subst c0 c s0 s3 -> map fst s0 = map fst c.
-Proof.
-  induction 1;
-    basic_goal_prep;
-    basic_core_crush.
-Qed.
-#[local] Hint Rewrite eq_subst_map_fst_l using eassumption : lang_core.
-
-
-Lemma eq_subst_fresh_r c0 c s0 s3 n
-  : eq_subst c0 c s0 s3 -> fresh n c -> fresh n s3.
-Proof.
-  unfold fresh; intros.
-  erewrite eq_subst_map_fst_r; eauto.
-Qed.
-#[local] Hint Resolve eq_subst_fresh_r : lang_core.
-
-Lemma eq_subst_fresh_l c0 c s0 s3 n
-  : eq_subst c0 c s0 s3 -> fresh n c -> fresh n s0.
-Proof.
-  unfold fresh; intros.
-  erewrite eq_subst_map_fst_l; eauto.
-Qed.
-#[local] Hint Resolve eq_subst_fresh_l : lang_core.
-
-Lemma ctx_admissible_in c n t
-  : wf_ctx c ->
-    ctx_cut_admissible c ->
-    In (n, t) c ->
-    sort_cut_admissible c t t.
-Proof.
-  induction 1;
-    basic_goal_prep;
-    basic_core_crush.
-  {
-    clear H3.
-    unfold sort_cut_admissible in *;
-      intros.
-    safe_invert H2.
-    erewrite !strengthen_subst;
-      try typeclasses eauto;
-      eauto.
-    all: basic_core_crush.
-  }
-  {
-    clear H4.      
-    unfold sort_cut_admissible in *;
-      intros.
-    safe_invert H3.
-    erewrite !strengthen_subst;
-      try typeclasses eauto;
-      eauto.
-    all: basic_core_crush.
-  }
-Qed.
-    
-    
+  Qed.    
   
+  Hint Resolve ctx_lang_mono : lang_core.
+  
+  Lemma rule_mono r : wf_rule l r -> wf_rule l' r.
+  Proof.
+    destruct 1;
+      basic_goal_prep;
+      basic_core_crush.
+  Qed.  
+
+End LangMono.
+
+
+
+
+
+Inductive wf_lang : lang -> Prop :=
+| wf_lang_nil : wf_lang []
+| wf_lang_cons : forall l n r,
+    fresh n (l) ->
+    wf_lang l ->
+    wf_rule (l) r ->
+    wf_lang ((n,r)::l).
+
+
+Lemma wf_lang_implies_ws l
+  : wf_lang l -> ws_lang l.
+Proof.
+  induction 1;
+    basic_goal_prep;
+    basic_core_crush.
+Qed.
+Hint Resolve wf_lang_implies_ws : lang_core.
+
+
+
+Lemma rule_in_wf l name r
+  : wf_lang l -> In (name, r) l -> wf_rule l r.
+Proof.
+  induction 1;
+    basic_goal_prep;
+    [tauto|].
+  eapply rule_mono; cycle 1;
+    basic_core_crush.
+Qed.
+Hint Resolve rule_in_wf : lang_core.
+
+Local Ltac use_rule_in_wf :=
+  lazymatch goal with
+  | H:wf_lang ?l, Hin:In (_, _) ?l |- _ => pose proof (rule_in_wf _ _ _ H Hin)
+  end.
+
+Section WithLang.
+  Context (l : lang)
+    (wfl : wf_lang l).
+
+  Local Notation wf_ctx c := (wf_ctx l c).
+  Local Notation eq_sort c' t1' t2' := (eq_sort l c' t1' t2').
+  Local Notation eq_term c' t e1 e2 := (eq_term l c' t e1 e2).
+  Local Notation eq_subst c c' s1' s2' := (eq_subst l c c' s1' s2').
+  Local Notation eq_args c c' s1' s2' := (eq_args l c c' s1' s2').
+  
+  Local Notation weak_sort_cut_admissible c' t1' t2' := (weak_sort_cut_admissible l c' t1' t2').
+  Local Notation weak_term_cut_admissible c' t e1 e2 := (weak_term_cut_admissible l c' t e1 e2).
+  Local Notation weak_subst_cut_admissible c c' s1' s2' := (weak_subst_cut_admissible l c c' s1' s2').
+  Local Notation weak_args_cut_admissible c c' s1' s2' := (weak_args_cut_admissible l c c' s1' s2').
+
+  Context (Hla : all (rule_cut_admissible l) (map snd l)).
+  Context (c : ctx).
+  Context (wfc : wf_ctx c).
+  Context (Hca : ctx_cut_admissible l c).
+
   Lemma weak_cut_admissible
-    : (forall c' t1' t2',
-          eq_sort c' t1' t2' ->
-          weak_sort_cut_admissible c' t1' t2'
-             /\ weak_sort_cut_admissible c' t1' t1'
-             /\ weak_sort_cut_admissible c' t2' t2')
-      /\ (forall c' (t : Term.sort V) (e1 e2 : Term.term V),
-             eq_term c' t e1 e2 ->
-             weak_term_cut_admissible c' t e1 e2
-             /\ weak_term_cut_admissible c' t e1 e1
-             /\ weak_term_cut_admissible c' t e2 e2
-             /\ weak_sort_cut_admissible c' t t)
-      /\ ((*wf_lang l ->*)
-          forall (c c' : Term.ctx V) (s1 s2 : Term.subst V),
+    : (forall t1' t2',
+          eq_sort c t1' t2' ->
+          weak_sort_cut_admissible c t1' t2'
+             /\ weak_sort_cut_admissible c t1' t1'
+             /\ weak_sort_cut_admissible c t2' t2')
+      /\ (forall (t : Term.sort V) (e1 e2 : Term.term V),
+             eq_term c t e1 e2 ->
+             weak_term_cut_admissible c t e1 e2
+             /\ weak_term_cut_admissible c t e1 e1
+             /\ weak_term_cut_admissible c t e2 e2
+             /\ weak_sort_cut_admissible c t t)
+      /\ (forall (c' : Term.ctx V) (s1 s2 : Term.subst V),
             eq_subst c c' s1 s2 ->
             weak_subst_cut_admissible c c' s1 s2
             /\ weak_subst_cut_admissible c c' s1 s1
             /\ weak_subst_cut_admissible c c' s2 s2)
-      /\ (forall c c' (s1 s2 : list term),
+      /\ (forall c' (s1 s2 : list term),
             eq_args c c' s1 s2 ->
             weak_args_cut_admissible c c' s1 s2
             /\ weak_args_cut_admissible c c' s1 s1
@@ -787,6 +1076,7 @@ Qed.
     simple eapply cut_ind.
     all: unfold weak_term_cut_admissible, weak_sort_cut_admissible, weak_subst_cut_admissible, weak_args_cut_admissible.
     all: basic_goal_prep.
+    all: try use_rule_in_wf; autorewrite with lang_core utils in *.
     all: repeat split.
     all: basic_goal_prep.
     all: erewrite ?subst_assoc; try typeclasses eauto;[|shelve..].
@@ -796,28 +1086,22 @@ Qed.
         eapply in_all_named_list in lang_admissible; eauto;
         cbn in lang_admissible
     end.
-    all: eauto with lang_core.
-    1: basic_core_crush.
-    1: basic_core_crush.
-    1: basic_core_crush.
-    1: basic_core_crush.
-    1: basic_core_crush.
+    all: try now intuition eauto with lang_core.
     {
-      eapply eq_term_conv.
-      {
-        basic_core_crush.
-      }
-      {
-        basic_core_crush.
-      }
+      eapply eq_sort_trans; intuition eauto using eq_sort_by, eq_subst_refl_right.
     }
-    1:basic_core_crush.
-    1:basic_core_crush.
+    {
+      eapply eq_sort_sym; intuition eauto using eq_subst_refl_right, eq_subst_sym'.
+    }
+    {
+      eapply eq_term_conv;
+        try now intuition eauto with lang_core.
+      eapply Hla;  intuition eauto using eq_subst_refl_right.
+    }
     {
       rewrite <- !Substable.with_names_from_args_subst.
       eapply eq_term_cong; eauto.
       eapply H1; intuition eauto.
-      basic_core_crush.
     }
     {
       rewrite <- !Substable.with_names_from_args_subst.
@@ -825,14 +1109,12 @@ Qed.
       {
         eapply eq_term_cong; eauto.
         eapply H2; intuition eauto.
-        basic_core_crush.
       }
       {
-        eapply lang_admissible; eauto.
-        2:basic_core_crush.
+        eapply Hla; eauto.
         eapply eq_args_implies_eq_subst.
         eapply H1; eauto.
-        all: intuition eauto with lang_core.
+        all: intuition eauto using eq_subst_refl_right with lang_core.
       }     
     }
     {
@@ -841,130 +1123,119 @@ Qed.
       {
         eapply eq_term_cong; eauto.
         eapply H3; intuition eauto.
-        basic_core_crush.
       }
       {
-        eapply lang_admissible; eauto.
-        2:basic_core_crush.
+        eapply Hla; eauto.
         eapply eq_args_implies_eq_subst.
         eapply H3; intuition eauto.
-        all: eauto with lang_core.
+        all: intuition eauto using eq_subst_refl_right with lang_core.
       }     
     }
     {
-      eapply lang_admissible.
+      eapply Hla.
       2:basic_core_crush.
       rewrite <- !Substable.with_names_from_args_subst.
       eapply eq_args_implies_eq_subst.
       eapply H3; intuition eauto.
-      all: eauto with lang_core.
     }
     {
-      eapply ctx_admissible_in; eauto.
+      eapply ctx_admissible_in; eauto with lang_core.
+    }
+    {
+      eapply eq_term_trans; intuition eauto using eq_sort_by, eq_subst_refl_right.
     }
     {
       eapply eq_term_sym.
       eapply eq_term_conv; eauto using eq_subst_sym'.
     }
-    {
-      constructor.
-      {
-        basic_core_crush.
-      }
-      {
-        replace t [/s2 [/s2' /] /] with t [/s2 /] [/s2' /]; eauto.
-        erewrite subst_assoc; try typeclasses eauto; eauto.
-        basic_core_crush.
-      }
-    }
-    {
-      constructor.
-      {
-        basic_core_crush.
-      }
-      {
-        eapply eq_term_conv.
-        {
-          basic_core_crush.
-        }
-        {
-          erewrite subst_assoc; try typeclasses eauto; eauto.
-          2:basic_core_crush.
-          fold_Substable.
-          safe_invert H10.
-          eauto using eq_subst_sym', eq_subst_refl_right.
-        }
-      }
-    }      
-    {
-      constructor.
-      {
-        basic_core_crush.
-      }
-      {
-        eapply eq_term_conv.
-        {
-          basic_core_crush.
-        }
-        {
-          erewrite subst_assoc; try typeclasses eauto; eauto.
-          2:basic_core_crush.
-          fold_Substable.
-          safe_invert H10.
-          eauto using eq_subst_sym', eq_subst_refl_right.
-        }
-      }
-    }
-    all: constructor; [basic_core_crush|].
+    1-3:eapply eq_term_conv; now eauto using eq_subst_refl_right.
+    all: constructor; eauto.
     all: eapply eq_term_conv; [basic_core_crush|].
-    {
-      rewrite !Substable.with_names_from_args_subst.
-      unfold apply_subst at 4.
-      unfold substable_subst.      
-      erewrite <- subst_assoc; try typeclasses eauto; eauto.
+    all: unfold sort_cut_admissible in *.
+    1-3: erewrite subst_assoc; try typeclasses eauto; eauto;
+    erewrite ?eq_subst_map_fst_r by eassumption;
+    [|basic_core_crush].
+    all: fold_Substable.
+    all:eauto using eq_subst_sym', eq_subst_refl_right,eq_args_implies_eq_subst.
+    2:{
+      erewrite subst_assoc; try typeclasses eauto; eauto using eq_subst_refl_right.
       {
-        eapply H5; eauto using eq_subst_refl_right.
+        fold_Substable.
+        eapply H11; eauto.
+        rewrite <- !Substable.with_names_from_args_subst.
+        eapply eq_subst_sym'; eauto.
+        eapply eq_args_implies_eq_subst.
+        eauto using eq_subst_refl_right.
       }
-      basic_core_crush.
+      rewrite ?map_fst_with_names_from.
+      1:basic_core_crush.
+      erewrite eq_args_len_eq_r; eauto.
     }
-    {
-      erewrite subst_assoc; try typeclasses eauto; eauto.
-      2:{
-        basic_core_crush.
-      }
-      eapply H11.
-      2:basic_core_crush.
-      fold_Substable.
-      rewrite <- !Substable.with_names_from_args_subst.
-      eapply eq_subst_sym'; eauto; [|basic_core_crush].
-      eapply eq_args_implies_eq_subst.
-      basic_core_crush.
-    }
-    {
-      erewrite subst_assoc; try typeclasses eauto; eauto.
-      2:{
-        basic_core_crush.
-      }
-      eapply H11.
-      2:basic_core_crush.
-      fold_Substable.
-      rewrite <- !Substable.with_names_from_args_subst.
-      eapply eq_args_implies_eq_subst.
-      basic_core_crush.
-    }
-
-
+    all: rewrite !Substable.with_names_from_args_subst.
+    all: unfold apply_subst at 4.
+    all: unfold substable_subst.      
+    all: erewrite <- subst_assoc; try typeclasses eauto; eauto using eq_subst_refl_right.
     Unshelve.
     all: rewrite ?map_fst_with_names_from.
     all: erewrite ?eq_subst_map_fst_r by eassumption.
     all: erewrite ?eq_subst_map_fst_l by eassumption.
     all: eauto with lang_core.
-    all: use_rule_in_wf.
-    all: autorewrite with utils lang_core in *.
-    all: break.
-    all: eauto with lang_core.
-  Qed.    
-           
+    all: erewrite eq_args_len_eq_r; eauto.
+  Qed.
+
+  Lemma ctx_cut_admissible c
+    : wf_ctx c ->
+      ctx_cut_admissible c.
+  Proof.
+    induction 1;
+      basic_goal_prep
+      
+      /\ (forall c c' (s1 s2 : list term),
+            eq_args c c' s1 s2 ->
+            weak_args_cut_admissible c c' s1 s2
+            /\ weak_args_cut_admissible c c' s1 s1
+            /\ weak_args_cut_admissible c c' s2 s2).
+
+
+
+  Context (wfl : wf_lang l).
+  
+  Local Lemma cut_implies_core 
+    : (forall c t1 t2,
+          eq_sort c t1 t2 ->
+          Core.eq_sort l c t1 t2)
+      /\ (forall c t e1 e2,
+             eq_term c t e1 e2 ->
+             Core.eq_term l c t e1 e2)
+      /\ (forall c c' s1 s2,
+             eq_subst c c' s1 s2 ->
+             Model.eq_subst (Model := core_model l) c c' s1 s2)
+      /\ (forall c c' s1 s2,
+             eq_args c c' s1 s2 ->
+             Model.eq_args (Model := core_model l) c c' s1 s2).
+  Proof using V_Eqb_ok wfl.
+    simple eapply cut_ind;
+      basic_goal_prep;
+      basic_core_crush.
+    all: eauto using
+           sort_con_congruence,
+        Core.eq_sort_trans, Core.eq_sort_sym,
+        term_con_congruence,
+        Core.eq_term_trans, Core.eq_term_sym.
+  Qed.
+
+  Definition eq_sort_cut_implies_core := proj1 cut_implies_core.
+  Local Hint Resolve eq_sort_cut_implies_core : lang_core.
+  
+  Definition eq_term_cut_implies_core := proj1 (proj2 cut_implies_core).
+  Local Hint Resolve eq_term_cut_implies_core : lang_core.
+
+  Definition eq_subst_cut_implies_core := proj1 (proj2 (proj2 cut_implies_core)).
+  Local Hint Resolve eq_subst_cut_implies_core : lang_core.
+  
+  Definition eq_args_cut_implies_core := proj2 (proj2 (proj2 cut_implies_core)).
+  Local Hint Resolve eq_args_cut_implies_core : lang_core.
+    
   Lemma core_implies_cut
     : (forall c t1 t2,
           Core.eq_sort l c t1 t2 ->
@@ -1019,7 +1290,6 @@ Qed.
   Qed.
   
   
-End Terms.
 
 (* TODO: assess benefits of retaining symmetry, transitivity
 Hint Constructors eq_sort eq_term eq_subst eq_args
